Change in the validator to check the "mask/jump" pseudo instruction in one call
The use of an option register was really a pain for the inductions

NTCB/Validator.v
@@ -16,7 +16,7 @@ Module ValidatorCode (Import I: INSTRUCTION).
 
   Definition id (n: nat) := n.
 
-  Function validate_n_byte (n: nat) (oreg: option register) (addr: N)
+  Function validate_n_byte (n: nat) (addr: N)
     (valid_addresses to_be_checked_addresses: NSet) (ll: lazy_list byte)
     {measure id n}: option (NSet * NSet * lazy_list byte):=
     match n with
@@ -28,54 +28,74 @@ Module ValidatorCode (Import I: INSTRUCTION).
         let addr' := addr + (N_of_nat size_instr) in
         match classify_instruction instr with
           | OK_instr =>
-            validate_n_byte n' None addr'
+            validate_n_byte n' addr'
               (Nadd addr valid_addresses) to_be_checked_addresses ll'
-          | Mask_instr reg w =>
+          | Mask_instr reg1 w =>
             match word_eq_dec w proper_mask with
               | left _ =>
-                validate_n_byte n' (Some reg)
-                addr' (Nadd addr valid_addresses) to_be_checked_addresses ll'
+                (* if we are masking with the right mask, we check the next instruction*)
+                match n' with
+                  | O => Some (Nadd addr valid_addresses, to_be_checked_addresses, ll') 
+                  | _ =>
+                    do (instr', size_instr') <- parse_instruction (byte_map_from_ll ll');
+                    match classify_instruction instr' with
+                      | Indirect_jump reg2 => (* an indirect jump *)
+                        match register_eq_dec reg1 reg2 with
+                          | left _ => (* the proper register *)
+                            do ll'' <- ll_safe_drop size_instr' ll';
+                            do n'' <- safe_minus n' size_instr';
+                            let addr'' := addr' + (N_of_nat size_instr') in
+                            validate_n_byte n'' addr''
+                              (Nadd addr valid_addresses) to_be_checked_addresses ll''
+                          | right _ => None
+                        end
+                      | _ =>
+                        validate_n_byte n' addr'
+                          (Nadd addr valid_addresses) to_be_checked_addresses ll'
+                    end
+                end
               | right _ =>
-                validate_n_byte n' None
-                addr' (Nadd addr valid_addresses) to_be_checked_addresses ll'
+                validate_n_byte n'
+                  addr' (Nadd addr valid_addresses) to_be_checked_addresses ll'
             end
           | Direct_jump w =>
             let dest_addr := N_of_word w in
             if dividable_by_32_dec dest_addr then
-              validate_n_byte n' None
-                addr' (Nadd addr valid_addresses) to_be_checked_addresses ll'
+              validate_n_byte n' addr'
+                (Nadd addr valid_addresses) to_be_checked_addresses ll'
             else if is_Nin dest_addr valid_addresses then
-              validate_n_byte n' None
-                addr' (Nadd addr valid_addresses) to_be_checked_addresses ll'
+              validate_n_byte n' addr'
+                (Nadd addr valid_addresses) to_be_checked_addresses ll'
             else
-              validate_n_byte n' None addr' (Nadd addr valid_addresses)
+              validate_n_byte n' addr' (Nadd addr valid_addresses)
                 (Nadd dest_addr to_be_checked_addresses) ll'
-          | Indirect_jump reg2 =>
-            do reg1 <- oreg;
-            match register_eq_dec reg1 reg2 with
-              | left _ =>
-                validate_n_byte n' None
-                addr' valid_addresses to_be_checked_addresses ll'
-              | right _ => None
-            end
-          | Invalid_instruction => None
+          | Invalid_instruction
+          | Indirect_jump _ => None
         end
     end.
   Proof.
-
-    Ltac solve_case teq0 teq3 := solve [
-      intros;
-      pose proof (size_instr_not_0 teq0);
-      apply safe_minus_correct in teq3; subst;
-      unfold id; omega].
-
-    solve_case teq0 teq3.
-    solve_case teq0 teq3.
-    solve_case teq0 teq3.
-    solve_case teq0 teq3.
-    solve_case teq0 teq3.
-    solve_case teq0 teq3.
-    solve_case teq0 teq3.
+    Ltac solve_case :=
+    intros;
+    repeat
+      match goal with
+        | H : parse_instruction _ = Some _ |- _ =>
+          apply size_instr_not_0 in H
+      end;
+    repeat
+      match goal with
+        | H: safe_minus _ _ = _ |- _ =>
+          apply safe_minus_correct in H
+      end; subst; unfold id; omega.
+    solve_case.
+    solve_case.
+    solve_case.
+    solve_case.
+    solve_case.
+    solve_case.
+    solve_case.
+    solve_case.
+    solve_case.
+    solve_case.
   Qed.
  
   Ltac fun_ind_validate_n_byte_with call :=
@@ -93,27 +113,34 @@ Module ValidatorCode (Import I: INSTRUCTION).
       | fst_Case_tac "fun_ind_validate_n_byte 11"
       | fst_Case_tac "fun_ind_validate_n_byte 12"
       | fst_Case_tac "fun_ind_validate_n_byte 13"
-      | fst_Case_tac "fun_ind_validate_n_byte 14"].
+      | fst_Case_tac "fun_ind_validate_n_byte 14"
+      | fst_Case_tac "fun_ind_validate_n_byte 15"
+      | fst_Case_tac "fun_ind_validate_n_byte 16"
+      | fst_Case_tac "fun_ind_validate_n_byte 17"
+      | fst_Case_tac "fun_ind_validate_n_byte 18"].
 
   Ltac fun_ind_validate_n_byte :=
     match goal with
-      | |- context[ validate_n_byte ?n ?or ?a ?va ?tbca ?ll] =>
+      | |- context[ validate_n_byte ?n ?a ?va ?tbca ?ll] =>
         fun_ind_validate_n_byte_with
-          (validate_n_byte n or a va tbca ll)
+          (validate_n_byte n a va tbca ll)
     end.
 
   Lemma validate_n_byte_reduces_size_by_n:
-    forall n oreg addr valid_addresses to_be_checked_addresses ll
+    forall n addr valid_addresses to_be_checked_addresses ll
       valid_addresses' to_be_checked_addresses' ll',
-      validate_n_byte n oreg addr valid_addresses to_be_checked_addresses ll =
+      validate_n_byte n addr valid_addresses to_be_checked_addresses ll =
       Some (valid_addresses', to_be_checked_addresses', ll') ->
       ll_length ll = (n + ll_length ll')%nat.
   Proof.
     intros ? ? ? ? ? ?.
     fun_ind_validate_n_byte;
-      intros; clean; specialize (IHo _ _ _ H);
+      intros; clean;
+        try (specialize (IHo _ _ H));
         apply ll_safe_drop_size in  e2;
-          apply safe_minus_correct in e3; omega.
+          apply safe_minus_correct in e3; try omega.
+    apply ll_safe_drop_size in e11. apply safe_minus_correct in e12.
+    subst. omega.
   Qed.
 
 
@@ -121,7 +148,7 @@ Module ValidatorCode (Import I: INSTRUCTION).
     (valid_addresses to_be_checked_addresses: NSet) (ll: lazy_list byte)
     {measure ll_length ll}: option (NSet * NSet):=
     do (valid_addresses', to_be_checked_addresses', ll') <-
-      validate_n_byte 32 None addr valid_addresses to_be_checked_addresses ll;
+      validate_n_byte 32 addr valid_addresses to_be_checked_addresses ll;
     match ll' with
       | 〈〉 => Some (valid_addresses', to_be_checked_addresses')
       | _ =>
