NTCB/ValidatorProof.v
@@ -17,12 +17,12 @@ Module ValProof (Import I : INSTRUCTION) (Import ISP: INSTRUCTION_SEMANTICS_PROP
   Import Val.
   Ltac fun_ind_validate_n_byte :=
     match goal with
-      | |- context[ validate_n_byte ?n ?or ?a ?va ?tbca ?ll] =>
+      | |- context[ validate_n_byte ?n ?a ?va ?tbca ?ll] =>
         fun_ind_validate_n_byte_with
-          (validate_n_byte n or a va tbca ll)
-      | H : context[ validate_n_byte ?n ?or ?a ?va ?tbca ?ll] |- _ =>
+          (validate_n_byte n a va tbca ll)
+      | H : context[ validate_n_byte ?n ?a ?va ?tbca ?ll] |- _ =>
         fun_ind_validate_n_byte_with
-          (validate_n_byte n or a va tbca ll)
+          (validate_n_byte n a va tbca ll)
     end.
 
   Ltac fun_ind_validate_ll_with call :=
@@ -43,10 +43,10 @@ Module ValProof (Import I : INSTRUCTION) (Import ISP: INSTRUCTION_SEMANTICS_PROP
 
 
   Lemma validate_n_byte_increase_valid_addresses:
-    forall (n: nat) (oreg: option register) (addr: N)
+    forall (n: nat) (addr: N)
     (valid_addresses to_be_checked_addresses: NSet) (ll: lazy_list byte)
     valid_addresses' to_be_checked_addresses' ll',
-    validate_n_byte n oreg addr valid_addresses to_be_checked_addresses ll =
+    validate_n_byte n addr valid_addresses to_be_checked_addresses ll =
     Some (valid_addresses', to_be_checked_addresses', ll') ->
     Nincluded valid_addresses valid_addresses'.
   Proof.
@@ -55,10 +55,10 @@ Module ValProof (Import I : INSTRUCTION) (Import ISP: INSTRUCTION_SEMANTICS_PROP
   Qed.
 
   Lemma validate_n_byte_increase_to_be_checked_addresses:
-    forall (n: nat) (oreg: option register) (addr: N)
+    forall (n: nat) (addr: N)
     (valid_addresses to_be_checked_addresses: NSet) (ll: lazy_list byte)
     valid_addresses' to_be_checked_addresses' ll',
-    validate_n_byte n oreg addr valid_addresses to_be_checked_addresses ll =
+    validate_n_byte n addr valid_addresses to_be_checked_addresses ll =
     Some (valid_addresses', to_be_checked_addresses', ll') ->
     Nincluded to_be_checked_addresses to_be_checked_addresses'.
   Proof.
@@ -78,10 +78,10 @@ Module ValProof (Import I : INSTRUCTION) (Import ISP: INSTRUCTION_SEMANTICS_PROP
 
 
   Lemma validate_n_byte_drop_n:
-    forall (n: nat) (oreg: option register) (addr: N)
+    forall (n: nat) (addr: N)
     (valid_addresses to_be_checked_addresses: NSet) (ll: lazy_list byte)
     valid_addresses' to_be_checked_addresses' ll',
-    validate_n_byte n oreg addr valid_addresses to_be_checked_addresses ll =
+    validate_n_byte n addr valid_addresses to_be_checked_addresses ll =
     Some (valid_addresses', to_be_checked_addresses', ll') ->
     ll_safe_drop n ll = Some ll'.
   Proof.
@@ -89,6 +89,8 @@ Module ValProof (Import I : INSTRUCTION) (Import ISP: INSTRUCTION_SEMANTICS_PROP
     fun_ind_validate_n_byte; clean; eauto with nset;
     apply safe_minus_correct in e3; subst;
     rewrite ll_safe_drop_plus; rewrite e2; eauto.
+    apply safe_minus_correct in e12.
+    subst. rewrite ll_safe_drop_plus; rewrite e11; eauto.
   Qed.
   Local Hint Resolve validate_n_byte_drop_n validate_n_byte_increase_to_be_checked_addresses
     validate_n_byte_increase_valid_addresses.
@@ -125,35 +127,41 @@ Module ValProof (Import I : INSTRUCTION) (Import ISP: INSTRUCTION_SEMANTICS_PROP
     forall (addr: N) n
     (valid_addresses to_be_checked_addresses: NSet) (ll: lazy_list byte)
     valid_addresses' to_be_checked_addresses' ll',
-    validate_n_byte (S n) None addr valid_addresses to_be_checked_addresses ll =
+    validate_n_byte (S n) addr valid_addresses to_be_checked_addresses ll =
     Some (valid_addresses', to_be_checked_addresses', ll') ->
     In_NSet addr valid_addresses'.
   Proof.
     intros * VALIDATE.
-    functional inversion VALIDATE; subst;
-    subst;
+    functional inversion VALIDATE; try (subst;
+    subst);
     repeat match goal with
       | x := _ : _ |- _ => subst x
     end;
-    apply validate_n_byte_increase_valid_addresses in X;
+    (try apply validate_n_byte_increase_valid_addresses in X);
     eauto with nset.
   Qed.
 
   Local Hint Resolve validate_n_byte_add_addr.
 
   Lemma validate_n_byte_size:
-    forall (n: nat) (oreg: option register) (addr: N)
+    forall (n: nat) (addr: N)
     (valid_addresses to_be_checked_addresses: NSet) (ll: lazy_list byte)
     valid_addresses' to_be_checked_addresses',
-    validate_n_byte n oreg addr valid_addresses to_be_checked_addresses ll =
+    validate_n_byte n addr valid_addresses to_be_checked_addresses ll =
     Some (valid_addresses', to_be_checked_addresses', 〈〉) ->
     ll_length ll = n.
   Proof.
     intros * VALIDATE.
     fun_ind_validate_n_byte; clean;
-    specialize (IHo VALIDATE); subst;
+    try (specialize (IHo VALIDATE)); subst;
     apply ll_safe_drop_size in e2;
-    apply safe_minus_correct in e3; omega.
+    apply safe_minus_correct in e3; try omega.
+
+    Case "fun_ind_validate_n_byte 3".
+    simpl in *. omega.
+    Case "fun_ind_validate_n_byte 4".
+    apply ll_safe_drop_size in e11.
+    apply safe_minus_correct in e12. omega.
   Qed.
 
   Ltac omega' := zify; omega.
@@ -170,11 +178,11 @@ Module ValProof (Import I : INSTRUCTION) (Import ISP: INSTRUCTION_SEMANTICS_PROP
     intros *.
     fun_ind_validate_ll; intros; clean; eauto.
     Case "fun_ind_validate_ll 1".
-      pose proof (validate_n_byte_size _ _ _ _ _ _ _ _ e).
+      pose proof (validate_n_byte_size _ _ _ _ _ _ _ e).
       apply validate_n_byte_add_addr in e.
       replace addr' with addr. assumption.
       rewrite H0 in H2. simpl in H2.
-      destruct H. destruct H3. zify. omega.
+      destruct H. destruct H3. omega'.
 
     Case "fun_ind_validate_ll 2".
       assert (dividable_by_32 (addr + 32)).
@@ -195,23 +203,23 @@ Module ValProof (Import I : INSTRUCTION) (Import ISP: INSTRUCTION_SEMANTICS_PROP
   Qed.
 
 
-Inductive ok_addr next_addr valid_addresses
-  to_be_checked_addresses addr : Prop :=
-| OA_Valid:
-  In_NSet addr valid_addresses ->
-  ok_addr next_addr valid_addresses to_be_checked_addresses addr
-| OK_checked:
-  In_NSet addr to_be_checked_addresses ->
-  ok_addr next_addr valid_addresses to_be_checked_addresses addr
-| OK_next: addr = next_addr ->
-  ok_addr next_addr valid_addresses to_be_checked_addresses addr
-| OK_div:
-  dividable_by_32 addr ->
-  ok_addr next_addr valid_addresses to_be_checked_addresses addr.
+  Inductive ok_addr next_addr valid_addresses
+    to_be_checked_addresses addr : Prop :=
+  | OA_Valid:
+    In_NSet addr valid_addresses ->
+    ok_addr next_addr valid_addresses to_be_checked_addresses addr
+  | OK_checked:
+    In_NSet addr to_be_checked_addresses ->
+    ok_addr next_addr valid_addresses to_be_checked_addresses addr
+  | OK_next: addr = next_addr ->
+    ok_addr next_addr valid_addresses to_be_checked_addresses addr
+  | OK_div:
+    dividable_by_32 addr ->
+    ok_addr next_addr valid_addresses to_be_checked_addresses addr.
   
 
-Inductive correct_addr mem next_addr valid_addresses
-  to_be_checked_addresses addr : Prop :=
+  Inductive correct_addr mem next_addr valid_addresses
+    to_be_checked_addresses addr : Prop :=
   | CA_intro:
     forall instr size_instr
     (SMALLER: addr + (N_of_nat size_instr) <= next_addr)
@@ -239,30 +247,30 @@ Inductive correct_addr mem next_addr valid_addresses
     correct_addr mem next_addr valid_addresses
       to_be_checked_addresses addr.
       
-Lemma correct_addr_same_code mem1 mem2
-  next_addr valid_addresses to_be_checked_addresses addr:
-  same_code next_addr mem1 mem2 ->
-  correct_addr mem1 next_addr valid_addresses to_be_checked_addresses addr ->
-  correct_addr mem2 next_addr valid_addresses to_be_checked_addresses addr.
-Proof.
-  intros SAME CORRECT.
-  inv CORRECT.
-  eapply' CA_intro; eauto.
-  Case "READ_FROM_MEM".
-    clear - SAME READ_FROM_MEM SMALLER.
-    unfold same_code, read_instr_from_memory in *.
-    eapply parse_instruction_only_read; eauto.
-    intros. simpl. apply SAME. omega'.
-  Case "CLASSIFY_MASK".
-    intros * OK.
-    specialize (CLASSIFY_MASK reg w OK).
-    destruct CLASSIFY_MASK as [|[instr' [size_instr' [?[? ?]]]]]; eauto.
-    right. exists instr'; exists size_instr'.
-    repeat split; eauto.
-    unfold same_code, read_instr_from_memory in *.
-    eapply parse_instruction_only_read; eauto.
-    intros. simpl. apply SAME. omega'.
-Qed.
+  Lemma correct_addr_same_code mem1 mem2
+    next_addr valid_addresses to_be_checked_addresses addr:
+    same_code next_addr mem1 mem2 ->
+    correct_addr mem1 next_addr valid_addresses to_be_checked_addresses addr ->
+    correct_addr mem2 next_addr valid_addresses to_be_checked_addresses addr.
+  Proof.
+    intros SAME CORRECT.
+    inv CORRECT.
+    eapply' CA_intro; eauto.
+    Case "READ_FROM_MEM".
+      clear - SAME READ_FROM_MEM SMALLER.
+      unfold same_code, read_instr_from_memory in *.
+      eapply parse_instruction_only_read; eauto.
+      intros. simpl. apply SAME. omega'.
+    Case "CLASSIFY_MASK".
+      intros * OK.
+      specialize (CLASSIFY_MASK reg w OK).
+      destruct CLASSIFY_MASK as [|[instr' [size_instr' [?[? ?]]]]]; eauto.
+      right. exists instr'; exists size_instr'.
+      repeat split; eauto.
+      unfold same_code, read_instr_from_memory in *.
+      eapply parse_instruction_only_read; eauto.
+      intros. simpl. apply SAME. omega'.
+  Qed.
 
 
   Definition correct_state_1 valid_addresses to_be_checked_addresses next_address (st: state register) :=
@@ -383,7 +391,7 @@ Qed.
     (valid_addresses to_be_checked_addresses: NSet) (ll: lazy_list byte)
     valid_addresses' to_be_checked_addresses' ll' oreg,
 
-    validate_n_byte n oreg addr valid_addresses to_be_checked_addresses ll =
+    validate_n_byte n addr valid_addresses to_be_checked_addresses ll =
       Some (valid_addresses', to_be_checked_addresses', ll') ->
     addr + (N_of_nat n) <= header_size + code_size ->
 
